mlir: proper tensor type, mainly

MLIRSemantics/SSAEnv.lean
@@ -23,96 +23,13 @@ edition.
 regions. Here again nothing prevents a region from shadowing variables or
 accessing out-of-scope values (in the case of an isolated region), but we only
 care when proving the correction of transformations.
-
-TODO:
- 1. How to guarantee that read values exist and have the proper type without
-    going too deep into proofs?
-    => Use default values! Data is always inhabited.
- 2. Improve the typing: auto-simplify τ.eval and the resulting casts
- 3. Set up infrastructure to unpack MLIRTy types into Lean native stuff
-
-Linking definitions and operations:
- 1. run (%a = 2) in environment env :: whatever
- 2. this returns () and env[%a=2] :: whatever
- 3. run (return %a) in environment env[%a=2] :: whatever
- 4. we can thus prove this returns 2
- 5. run (%b = %ext) in environment env[%a=2] :: whatever
- 6. result depends on whether %ext was defined in env, which we can't just
-    assume since we want theorems that work *in context*
-
-Value scoping: operation o1 dominates operation o2 if:
- - o2 is in the same block as o1 after o1, or
- - o2 is in a non-OpTrait::IsolatedFromAbove region dominated by o1
- - we don't handle concurrent semantics :x
-Block scoping: operation o1 can branch to block b2 if:
- - b2 is in the same region as the block owning o1
 -/
 
 import MLIRSemantics.Fitree
+import MLIRSemantics.Types
 
 import MLIR.AST
 open MLIR.AST
-
-
--- Additional definitions for MLIR.AST types
-
-instance: Coe String SSAVal where
-  coe := SSAVal.SSAVal
-
-def SSAVal.decEq (v1 v2: SSAVal): Decidable (Eq v1 v2) :=
-  match v1, v2 with
-  | SSAVal.SSAVal s1, SSAVal.SSAVal s2 =>
-      dite (s1 = s2)
-        (fun h => isTrue (by simp [h]))
-        (fun h => isFalse (by simp [h]))
-
-instance: DecidableEq SSAVal :=
-  SSAVal.decEq
-
-deriving instance DecidableEq for Dimension
-
-def MLIRTy.beq (t1 t2: MLIRTy): Bool :=
-  match t1, t2 with
-  | MLIRTy.fn a1 b1, MLIRTy.fn a2 b2 =>
-      beq a1 a2 && beq b1 b2
-  | MLIRTy.int n1, MLIRTy.int n2 =>
-      n1 == n2
-  | MLIRTy.float n1, MLIRTy.float n2 =>
-      n1 == n2
-  | MLIRTy.tuple [], MLIRTy.tuple [] =>
-      true
-  | MLIRTy.tuple (t1::l1), MLIRTy.tuple (t2::l2) =>
-      beq t1 t2 && beq (MLIRTy.tuple l1) (MLIRTy.tuple l2)
-  | MLIRTy.vector l1 t1, MLIRTy.vector l2 t2 =>
-      l1 == l2 && beq t1 t2
-  | MLIRTy.tensor l1 t1, MLIRTy.tensor l2 t2 =>
-      l1 == l2 && beq t1 t2
-  | MLIRTy.user n1, MLIRTy.user n2 =>
-      n1 == n2
-  | _, _ =>
-      false
-
-def MLIRTy.decEq (t1 t2: MLIRTy): Decidable (Eq t1 t2) :=
-  if MLIRTy.beq t1 t2 then isTrue sorry else isFalse sorry
-
-instance: DecidableEq MLIRTy :=
-  MLIRTy.decEq
-
-
--- Evaluation of MLIR types
--- TODO: Not all MLIRTy types are correctly evaluated
-
-@[simp, inline]
-def MLIR.AST.MLIRTy.eval: MLIRTy → Type
-  | MLIRTy.fn τ₁ τ₂ => τ₁.eval → τ₂.eval
-  | MLIRTy.int _ => Int
-  | MLIRTy.float _ => Float
-  | MLIRTy.tuple [] => Unit
-  | MLIRTy.tuple [τ] => τ.eval
-  | MLIRTy.tuple (τ::l) => τ.eval × (MLIRTy.tuple l).eval
-  | MLIRTy.vector _ _ => Unit /- todo -/
-  | MLIRTy.tensor _ _ => Unit /- todo -/
-  | MLIRTy.user _ => Unit /- todo -/
 
 
 -- SSAScope
@@ -170,8 +87,8 @@ def SSAEnv.set (name: SSAVal) (τ: MLIRTy) (v: τ.eval): SSAEnv → SSAEnv
 def SSAEnv.refines (new old: SSAEnv) :=
   ∀ ⦃name τ v⦄, old.get name τ = some v → new.get name τ = some v
 
-instance: LT SSAEnv where
-  lt := SSAEnv.refines -/
+instance: LE SSAEnv where
+  le := SSAEnv.refines -/
 
 
 -- Interactions manipulating the environment
@@ -189,19 +106,3 @@ def SSAEnvE.handle: SSAEnvE ~> StateT SSAEnv (Fitree PVoid) :=
         | none => return (default, env)
     | Set τ name v =>
         return ((), env.set name τ v)
-
-
--- Tests
-
-private def example_env (l: SSAScope) (s: SSAEnv): SSAEnv :=
-  (⟨"%0", MLIRTy.int 32, (42:Int)⟩ ::
-   ⟨"%1", MLIRTy.int 32, (7:Int)⟩ ::
-   l) ::
-  (⟨"%3", MLIRTy.int 32, (12:Int)⟩ ::
-   ⟨"%r", MLIRTy.float 32, (-1.7e3:Float)⟩ ::
-   []) ::
-  s
-
-example: ∀ l s, SSAEnv.get "%1" (MLIRTy.int 32) (example_env l s)
-    = some (7:Int) :=
-  by simp [cast_eq]
