MLIRSemantics/Toy/Toy.lean
@@ -1,39 +1,47 @@
 /- A toy dialect with basic tensor computations. -/
 
-def Vector (α: Type) (n: Nat) :=
-  Fin n → α
+import MLIRSemantics.Types
 
-def prod :=
-  List.foldl Nat.mul 1
 
--- Separate the vector and the equality proof so we can define the vector even
--- when dependent pattern matching fails to unify, and prove later
-structure Tensor (α: Type) (d: List Nat) where
-  size: Nat
-  data: Vector α size
-  H: size = prod d
+/-
+### Tensor reshaping operation
 
-/-===========-/
-/- Reshaping -/
-/-===========-/
+This operation can reshape (retype) tensors with fully-known dimensions,
+provided that the number of elements doesn't change.
+-/
 
-def reshape {α d} (d': List Nat) (H: prod d' = prod d):
-    Tensor α d → Tensor α d' :=
-  λ ⟨n, data, size⟩ => ⟨n, data, by rw [H]; assumption⟩
+def reshape {α} {D: DimList} (D': DimList)
+    (H: D.known) (H': D'.known) (Hprod: D'.prod = D.prod):
+    RankedTensor α D → RankedTensor α D' :=
+  fun t =>
+    { shape := D'.project,
+      size := t.size,
+      data := t.data,
+      Hdim := dim_known_project_refines H',
+      Hsize := by rw [t.Hsize, dim_known_prod D' H', Hprod]
+                  rw [dim_known_prod_refines H];
+                  apply t.Hdim }
 
-theorem reshape_reshape {α}:
-    ∀ d d' d'' (H': prod d' = prod d) (H'': prod d'' = prod d') (t: Tensor α d),
-    reshape d'' H'' (reshape d' H' t) = reshape d'' (Eq.trans H'' H') t := by
-  intros d d' d'' H' H'' t;
-  simp [reshape]
+theorem reshape_reshape {α} {D: DimList} (D₁ D₂: DimList)
+    (H: D.known) (H₁: D₁.known) (H₂: D₂.known)
+    (Hprod₁: D₁.prod = D.prod) (Hprod₂: D₂.prod = D₁.prod)
+    (t: RankedTensor α D):
+      reshape D₂ H₁ H₂ Hprod₂ (reshape D₁ H H₁ Hprod₁ t) =
+      reshape D₂ H H₂ (Eq.trans Hprod₂ Hprod₁) t :=
+  rfl
 
-theorem reshape_same {α}: ∀ d H (t: Tensor α d), reshape d H t = t := by
-  intros d H t;
-  simp [reshape]
+theorem reshape_self {α} D H₁ H₂ Hprod (t: RankedTensor α D):
+    reshape D H₁ H₂ Hprod t = t := by
+  simp [reshape, dim_known_project_eq H₁ t.Hdim]
 
-/-===============-/
-/- Transposition -/
-/-===============-/
+
+/-
+### Tensor transposition operation
+
+This operation shuffles the elements of the underlying data without changing
+its size. To keep this clean it's beneficial to separate the dimension logic
+from the index manipulation of the transposition itself.
+-/
 
 def transpose_remap (size n m: Nat) (H: size=n*m): Fin size → Fin size :=
   λ i =>
@@ -47,19 +55,31 @@ theorem transpose_remap_involutive (size n m H):
     = id := by
   simp [transpose_remap]
   funext i; apply Fin.eq_of_val_eq; simp
-  sorry
+  sorry /- fairly straightforward -/
 
-def transpose {α n m} (t: Tensor α [n,m]): Tensor α [m,n] :=
-  ⟨t.size,
-   t.data ∘ transpose_remap t.size n m (by simp [t.H, prod, List.foldl]),
-   by simp [t.H, prod, List.foldl, Nat.mul_comm]⟩
+@[inline]
+def Matrix α n m :=
+  RankedTensor α [MLIR.AST.Dimension.Known n, MLIR.AST.Dimension.Known m]
+
+def transpose {α n m} (t: Matrix α n m): Matrix α m n :=
+  { shape := [m, n],
+    size := t.size,
+    data := t.data ∘ transpose_remap t.size n m
+            (by rw [t.Hsize, dim_known_prod_refines _ t.Hdim] <;> simp),
+    Hdim := by simp,
+    Hsize := by simp [List.foldr];
+                rw [t.Hsize, dim_known_prod_refines _ t.Hdim] <;>
+                simp [Nat.mul_comm] }
 
 theorem Function.comp_assoc {α β γ δ} (f: α → β) (g: β → γ) (h: γ → δ):
     (h ∘ g) ∘ f = h ∘ (g ∘ f) :=
   by funext x; simp
 
 theorem transpose_involutive {α n m}:
-    ∀ (t: Tensor α [n,m]), transpose (transpose t) = t := by
-  intro ⟨size, data, H⟩;
+    ∀ (t: Matrix α n m), transpose (transpose t) = t := by
+  intro t;
   simp [transpose, Function.comp_assoc, transpose_remap_involutive]
-  funext i; simp
+  apply RankedTensor.eq_of_fields_eq <;> simp
+  . rw [←dim_known_project_eq _ t.Hdim] <;> simp
+  . simp [transpose]
+  . funext i; simp
