MLIRSemantics/Fitree.lean
@@ -1,3 +1,36 @@
+/-
+## Finite interaction trees
+
+The semantics framework for this project is extremely inspired by the Vellvm
+project [1] and is essentially centered around interaction trees and monadic
+transformers.
+
+Interactions trees are a particular instance of the freer monad; essentially,
+an ITree is a program that can have side effets through *interactions*, and
+these interactions can either be interpreted into the program or kept as
+observable side-effects.
+
+When giving semantics to a program, one usually starts with a rather simple
+ITree where most of the complex features of the language (memory, I/O,
+exceptions, randomness, non-determinism, etc) are hidden behind interactions.
+The interactions are then interpreted, which consists of (1) enriching the
+program's environment by a monadic transformation, and (2) replacing the
+interaction with an actual implementation.
+
+This approach allows monadic domains to be used while keeping each family of
+interactions separate. This is relevant for Vellvm as LLVM IR as many complex
+features, and even more relevant for MLIR since each dialect can bring more
+interactions and environment transforms and all of them have to be studied and
+defined independently.
+
+The datatype of interaction trees normally has built-in non-termination by
+being defined coinductively. Support for coinduction is still limited in Lean4,
+so we currently use a finite version of ITrees (hence called Fitree) which can
+only model programs that always terminate.
+
+[1]: https://github.com/vellvm/vellvm
+-/
+
 /- Extendable effect families -/
 
 section events
@@ -10,6 +43,7 @@ def psum (E: Type → Type u) (F: Type → Type v) :=
 inductive PVoid: Type -> Type u
 
 infixr:40 " ~> " => pto
+infixl:40 " +' " => psum
 
 class Member (E: Type → Type u) (F: Type → Type v) where
   inject : E ~> F
@@ -17,19 +51,19 @@ class Member (E: Type → Type u) (F: Type → Type v) where
 instance {E}: Member E E where
   inject := (fun _ => id)
 
-instance {E F G} [Member E F]: Member E (psum F G) where
+instance {E F G} [Member E F]: Member E (F +' G) where
   inject T := Sum.inl ∘ Member.inject T
 
-instance {E F G} [Member E G]: Member E (psum F G) where
+instance {E F G} [Member E G]: Member E (F +' G) where
   inject T := Sum.inr ∘ Member.inject T
 
 -- Effects can now be put in context automatically by typeclass resolution
 example (E: Type → Type u):
   Member E E := inferInstance
 example (E: Type → Type u) (F: Type → Type v):
-  Member E (psum E F) := inferInstance
+  Member E (E +' F) := inferInstance
 example (E: Type → Type u) (F: Type → Type v):
-  Member E (psum F (psum F E)) := inferInstance
+  Member E (F +' (F +' E)) := inferInstance
 
 end events
 
