MLIRSemantics/Toy/ToyDialect.lean
@@ -6,29 +6,52 @@ import MLIRSemantics.SSAEnv
 import MLIR.AST
 open MLIR.AST
 
-/- [Automatically generated] -/
+/- To be automatically generated -/
 
 inductive ToyOp: Type → Type _ :=
-  | Constant: (α: Type) → (n m: Nat) → Tensor α [n,m] →
-      ToyOp (Tensor α [n,m])
-  | Transpose: (α: Type) → (n m: Nat) → Tensor α [n,m] →
-      ToyOp (Tensor α [m,n])
-  | Reshape: (α: Type) → (n m n' m': Nat) → (H: n'*m' = n*m) → Tensor α [n,m] →
-      ToyOp (Tensor α [n',m'])
+  | Constant: (α: Type) → (n m: Nat) →
+      RankedTensor α [Dimension.Known n, Dimension.Known m] →
+      ToyOp (RankedTensor α [Dimension.Known n, Dimension.Known m])
+  | Transpose: (α: Type) → (n m: Nat) →
+      RankedTensor α [Dimension.Known n, Dimension.Known m] →
+      ToyOp (RankedTensor α [Dimension.Known m, Dimension.Known n])
+  | Reshape: (α: Type) → (D D': DimList) → (H: D.known) → (H': D'.known) →
+      (Hprod: D.prod = D'.prod) →
+      RankedTensor α D →
+      ToyOp (RankedTensor α D')
 
-/- Hopefully this could be automatically generated -/
+/- To be automatically generated -/
 
-def ToyOp.semantics: Op → Fitree (psum SSAEnvE ToyOp) Unit
-  | Op.mk "toy.constant" [] [] [] attributes
-        (MLIRTy.fn (MLIRTy.tuple []) _) =>
+def toy_semantics: Op → Fitree (psum SSAEnvE ToyOp) Unit
+  | Op.mk "toy.constant" [] [] [] attributes (MLIRTy.fn (MLIRTy.tuple []) _) =>
+      -- TODO: Access attributes
       return ()
-  | Op.mk "toy.transpose" [t_name] [] [] _ (MLIRTy.fn
-        (MLIRTy.tensor [Dimension.Known (n:Nat), Dimension.Known (m:Nat)] _) _) => do
-      /- TODO: Still need to model MLIR tensors -/
---      let t ← Fitree.trigger (@SSAEnvE.Get (Tensor Int [n,m]) _ t_name);
---      let t' ← Fitree.trigger (ToyOp.Transpose Int n m t);
-      return ()
+  | Op.mk "toy.transpose" [t_name] [] [] _ (MLIRTy.fn τ₁ τ₂) =>
+      match τ₁ with
+      | MLIRTy.tensor [Dimension.Known n, Dimension.Known m] τ => do
+          let t ← Fitree.trigger (@SSAEnvE.Get (MLIRTy.tensor [Dimension.Known
+                  n, Dimension.Known m] τ) _ t_name);
+          let t' ← Fitree.trigger (ToyOp.Transpose τ.eval n m t);
+          -- TODO: Have proper return names (ie. match above Op)
+          Fitree.trigger (@SSAEnvE.Set (MLIRTy.tensor [Dimension.Known m,
+            Dimension.Known n] τ) "%ret" t')
+      | _ =>
+          return ()
+  | Op.mk "toy.reshape" [t_name] [] [] _ (MLIRTy.fn τ₁ τ₂) =>
+      match τ₁, τ₂ with
+      | MLIRTy.tensor D σ₁, MLIRTy.tensor D' σ₂ =>
+          if σ₁ = σ₂ then do
+            let t ← Fitree.trigger (@SSAEnvE.Get (MLIRTy.tensor D σ₁) _ t_name);
+            -- TODO: Propagate verification invariants!
+            let t' ← Fitree.trigger (ToyOp.Reshape σ₁.eval D D'
+                     sorry sorry sorry sorry);
+            -- TODO: Cast σ₁ to σ₂?
+            Fitree.trigger (@SSAEnvE.Set (MLIRTy.tensor D' σ₁) "%ret" t')
+          else
+            return ()
+      | _, _ =>
+          return ()
   | _ =>
-      return ()
+      return () -- TODO: Maybe raise invalid instruction event for clarity?
 
 /- Manually specified: ToyOp event handler -/
