MLIRSemantics/Types.lean
@@ -1,0 +1,255 @@
+/-
+## MLIR types
+
+This file implements support for builtin MLIR types, as well as conversion to
+concrete Lean types and values.
+
+In order to support the untyped SSA environment (which doesn't require name
+definitions/uses to match as this is proven later), every concrete MLIR type
+should be Inhabited so that `SSAEnvE.Get` can return default values.
+
+Current properly-supported MLIR built-in types:
+
+* Function type [τ₁ → τ₂]: Lean function
+* Tuple type [(τ₁, ..., τₙ)]: n-ary product of underlying types
+* Tensors [tensor<DxDx?xDx?xτ>]: RankedTensor type
+
+Types that need improvements or refinements:
+
+* Unsigned finite integer types [u32, etc]
+  TODO: Model u32/etc with lean's Uint{8/16/32/64} or restart with Fin
+* Integer types [i32, etc]: currently use Int
+  TODO: Model i32/etc properly, probably restarting from Fin
+* Float types [f16, f32, f64, f80, f128]. todo
+  No idea how to model floats of different precisions in Lean?
+* Vectors: could expand on tensors. todo
+* Unranked tensors: todo
+* User types: should use a typeclass
+  TODO: Model user types
+-/
+
+import MLIRSemantics.Util.Arith
+
+import MLIR.AST
+open MLIR.AST
+
+
+/-
+### Vector types
+TODO: Not modeled fully by lean-mlir right now
+-/
+
+
+/-
+### Ranked tensors
+TODO: Consider a different type KnownRankedTensor that we could project to if
+TODO| we have known dimensions. Everything is conditioned by DimList.known...
+-/
+
+@[simp]
+def shape_prod :=
+  List.foldr (·*·) 1
+
+@[simp]
+def shape_refines: List Nat → List Dimension → Bool
+  | [], [] => true
+  | size::shape, Dimension.Unknown::dim => shape_refines shape dim
+  | size::shape, Dimension.Known d::dim => size = d && shape_refines shape dim
+  | (_::_), [] => false
+  | [], (_::_) => false
+
+@[inline]
+def DimList := List Dimension
+
+@[simp]
+def DimList.prod: DimList → Nat
+  | [] => 1
+  | Dimension.Known n :: D => n * prod D
+  | Dimension.Unknown :: _ => 0
+
+@[simp]
+def DimList.project: DimList → List Nat
+  | [] => []
+  | Dimension.Known n :: D => n :: project D
+  | Dimension.Unknown :: D => project D
+
+@[simp]
+def DimList.known: DimList → Bool
+  | [] => true
+  | Dimension.Known n :: D => known D
+  | Dimension.Unknown :: _ => false
+
+@[simp]
+def DimList.default_refinement: DimList → List Nat
+  | [] => []
+  | Dimension.Known n :: D => n :: default_refinement D
+  | Dimension.Unknown :: D => 0 :: default_refinement D
+
+theorem dim_known_project_refines {D: DimList}:
+    D.known → shape_refines D.project D := by
+  intros h <;> induction D <;> simp
+  case cons head tail ih =>
+    cases head <;> simp at *; apply (ih h)
+
+theorem dim_known_refines_inv {D: DimList} {S: List Nat}:
+    D.known → shape_refines S D → D = S.map Dimension.Known := by
+  intros Hknown; revert S; induction D <;> intros S Hrefines
+  case nil =>
+    cases S; simp [List.map]; simp at Hrefines
+  case cons head tail ih =>
+    cases S; simp at Hrefines
+    simp [List.map]; cases head <;> simp at *
+    rw [Hrefines.1, ←ih Hknown]; apply Hrefines.2
+
+theorem dim_known_project_eq {D: DimList}:
+    D.known → shape_refines S D → D.project = S := by
+  intros Hknown Hrefines
+  rw [dim_known_refines_inv Hknown Hrefines]
+  clear D Hknown Hrefines
+  induction S <;> simp; assumption
+
+theorem dim_known_prod_refines {D: DimList}:
+    D.known → shape_refines S D → shape_prod S = D.prod := by
+  intros Hknown; revert S; induction D <;> intros S Hrefines <;> simp
+  case nil =>
+    cases S; simp; simp at Hrefines
+  case cons head tail ih =>
+    cases S; simp at Hrefines
+    cases head <;> simp at *
+    rw [←Hrefines.1, ←ih Hknown Hrefines.2]
+    simp [List.foldr]
+
+theorem dim_known_prod (D: DimList):
+    D.known → shape_prod D.project = D.prod :=
+  fun Hknown =>
+    dim_known_prod_refines Hknown (dim_known_project_refines Hknown)
+
+theorem default_refinement_refines (D: DimList):
+    shape_refines D.default_refinement D := by
+  induction D <;> simp
+  case cons head _ ih =>
+    cases head <;> simp <;> apply ih
+
+-- Ranked tensors have known rank but possibly unknown dimensions. At runtime,
+-- the size is fully determined. We store the visible type information in the
+-- parameters of RankedTensor, and collect the fully-specified runtime data in
+-- the structure fields.
+--
+-- We add an intermediate [size] parameter so that we can separate data
+-- manipulation and proofs about the product of the dimensions, which would
+-- otherwise be tricky due to [Fin] constantly carrying proofs.
+structure RankedTensor (α: Type) (D: DimList) where
+  -- Actual dimensions
+  shape: List Nat
+  -- Contents; we use a function for brevity
+  -- TODO: RankedTensor: Consider a more computable data storage method
+  size: Nat
+  data: Fin size → α
+  -- Invariants: shape/dimension must be compatible, shape/size must match
+  Hdim: shape_refines shape D
+  Hsize: size = shape_prod shape
+
+theorem RankedTensor.eq_of_fields_eq (α D): ∀ (t₁ t₂: RankedTensor α D),
+  t₁.shape = t₂.shape →
+  (Hsize: t₁.size = t₂.size) →
+  (Hdata: HEq t₁.data t₂.data) →
+    t₁ = t₂ := by
+  intros t₁ t₂ Hshape Hsize Hdata
+  cases t₁; cases t₂; simp at *
+  trivial
+
+def RankedTensor.default {α D} [Inhabited α]: RankedTensor α D :=
+  { shape := D.default_refinement,
+    size  := shape_prod (D.default_refinement),
+    data  := fun _ => Inhabited.default,
+    Hdim  := default_refinement_refines _,
+    Hsize := rfl }
+
+instance {α D} [Inhabited α]: Inhabited (RankedTensor α D) where
+  default := RankedTensor.default
+
+/-
+### Unranked tensors
+TODO: Unranked tensors?
+-/
+
+/-
+### Evaluation of MLIR types
+TODO: Not all MLIRTy types are correctly evaluated
+-/
+
+/- MLIRTy is a nested inductive type, thus defined with well-founded recursion.
+   This prevents it from being reduced by the elaborator, so instead we define
+   it manually with the recursor.
+   See: https://leanprover.zulipchat.com/#narrow/stream/270676-lean4/topic/
+   reduction.20of.20dependent.20return.20type/near/276044057 -/
+
+@[reducible]
+def MLIR.AST.MLIRTy.eval (τ: MLIRTy): Type :=
+  @MLIRTy.rec
+    (motive_1 := fun _ => Type)
+    (motive_2 := fun _ => Type)
+    -- MLIRTy.fn
+    (fun τ₁ τ₂ eval_τ₁ eval_τ₂ => eval_τ₁ → eval_τ₂)
+    -- MLIRTy.int
+    (fun bitsize => Int)
+    -- MLIRTy.float
+    (fun bitsize => Float)
+    -- Mapping motive_2 to motive_1
+    (fun _ ih => ih)
+    -- MLIRTy.vector (todo)
+    (fun D τ eval_τ => Unit)
+    -- MLIRTy.tensor (todo)
+    (fun D τ eval_τ => RankedTensor eval_τ D)
+    -- MLIRTy.user (todo)
+    (fun name => Unit)
+    -- MLIRTy.tuple []
+    Unit
+    -- MLIRTy.tuple (τ::l)
+    (fun τ l eval_τ eval_l =>
+      match l with
+      | [] => eval_τ
+      | _  => eval_τ × eval_l)
+    τ
+
+@[reducible]
+def MLIR.AST.MLIRTy.evalList (l: List MLIRTy) : Type :=
+  @MLIRTy.rec_1
+    -- Same as above
+    (motive_1 := fun _ => Type)
+    (motive_2 := fun _ => Type)
+    (fun τ₁ τ₂ eval_τ₁ eval_τ₂ => eval_τ₁ → eval_τ₂)
+    (fun bitsize => Int)
+    (fun bitsize => Float)
+    (fun _ ih => ih)
+    (fun D τ eval_τ => Unit)
+    (fun D τ eval_τ => RankedTensor eval_τ D)
+    (fun name => Unit)
+    Unit
+    (fun τ l eval_τ eval_l =>
+      match l with
+      | [] => eval_τ
+      | _  => eval_τ × eval_l)
+    l
+
+mutual
+  def MLIR.AST.MLIRTy.default (τ: MLIRTy): τ.eval :=
+    match τ with
+    | MLIRTy.fn τ₁ τ₂ => (fun _ => τ₂.default)
+    | MLIRTy.int _ => (0:Int)
+    | MLIRTy.float _ => (0.0:Float)
+    | MLIRTy.tuple l => MLIRTy.defaultList l
+    | MLIRTy.vector _ _ => () /- todo -/
+    | MLIRTy.tensor D τ => @RankedTensor.default τ.eval D ⟨default τ⟩
+    | MLIRTy.user _ => () /- todo -/
+
+  protected def MLIR.AST.MLIRTy.defaultList (l: List MLIRTy):
+      MLIRTy.evalList l :=
+    match l with
+    | [] => ()
+    | [τ] => τ.default
+    | τ₁ :: τ₂ :: l => (τ₁.default, MLIRTy.defaultList (τ₂::l))
+end
+
+instance (τ: MLIRTy): Inhabited τ.eval where
+  default := τ.default
